The coefficients generated by this algorithm were independently validated 
against those for the $8^{th}$ order Gauss-Jackson algorithm presented by Berry 
and Healy~\cite{paper:Berry_Healy}.

\begin{enumerate}
 \item All \textit{predictor} coefficients match their analogous values 
 presented in Berry and Healy.
 \item All but one of the \textit{corrector} coefficients match; the exception 
 is the first element in the summed-adams corrector.
\end{enumerate}

Berry and Healy present the analogous $b_{44}$, used as:

\begin{equation*}
r_{n}=h\left(\nabla 
^{-1}\dot{r}_{n}-\frac{\dot{r}_{n}}{2}+b_{44}\dot{r}_{n}+\sum 
_{k=-4}^{3}b_{4k}(\dot{r}_{n+k-4})\right)
\end{equation*}

(see equations (68), (77))

We have, from equation~\ref{eq:sa_corr_form}:

\begin{equation*}
x_{n}=h\left(\nabla 
^{-1}{\dot{x}}_{n}+A_{\mathit{C0}}{\dot{x}}_{n}+\sum_{i=1}^{N}A_{Ci}{\dot{x}}_{n
-i})\right)
\end{equation*}

(which, with $i=4-k$, has identical form)

Consequently, we should expect:
$A_{\mathit{C0}}=b_{44}-\frac{1}{2}$,

Recalling from section~\ref{sec:math_form_summary_sa} (see, in particular, 
equation~\ref{eq:ACO_offset}) that the stored value for the first element of 
the summed-adams predictor coefficients is $1+A_{C0}$ rather than $A_{C0}$, we 
should expect to see that the stored value
\begin{equation*}
1+A_{\mathit{C0}}=b_{44}+\frac{1}{2} =  -\frac{63887}{89600}
\end{equation*}

which is observed.


All but one of the \textit{initializ} coefficients match with their 
analogous values presented in Berry and Healy; the exception is the fifth 
element in the summed-adams corrector, \textit{sa\_initializ\_coeff[4]}.

Berry and Healy present the analogous $b_{00}$, used as:

\begin{equation*}
\dot{r}_{0}=h\left(\nabla 
^{-1}{\ddot{r}}_{0}-\frac{{\ddot{r}}_{0}}{2}+\sum_{k=-4}^{-1}b_{0k}\ddot{r}_{k} 
+ b_{00}\ddot{r}_{0} + \sum_{k=1}^{4}b_{0k}\ddot{r}_{k} \right)
\end{equation*}
(see equation (69))


We have, from equation~\ref{eq:x0dot}, recognizing that order $N=8$ and that 
therefore the pre-/post- epoch split value $m = 4$:

\begin{equation*}
\dot{x}_{0}=h\left(\nabla 
^{-1}{\ddot{x}}_{0}+\sum_{i=0}^{3}A_{Ii}\ddot{x}_{4-i} + A_{I4}\ddot{x}_{0} + 
\sum_{i=4}^{8}A_{Ii}\ddot{x}_{4-i} \right)
\end{equation*}
(again, with $i=4-k$, these have identical form)

Consequently, we should expect:  
\begin{equation*}
A_{\mathit{I4}}=b_{00}-\frac{1}{2} = -\frac{1}{2}
\end{equation*}

which is observed.
